Symbol

NuPrime.thy
@@ -1,7 +1,7 @@
 (* KEEP IT SIMPLE AND STUPID *)
 
 theory NuPrime \<comment> \<open>The Primary Theory of the \<nu>-System\<close>
-  imports Main "HOL-Library.Monad_Syntax" NuHelpMath
+  imports Main "HOL-Library.Adhoc_Overloading" NuHelpMath
 begin
 
 text \<open>The fundamental theory for \<nu>-system\<close>
@@ -476,12 +476,12 @@ subsubsection \<open>Elementary instructions\<close>
 
 definition bind :: " ('a::lrep) state \<Rightarrow> ( 'a \<longmapsto> 'b) \<Rightarrow> ('b::lrep) state " \<comment>\<open>monadic bind\<close>
   where "bind s f = (case s of Success x \<Rightarrow> f x | Fail \<Rightarrow> Fail | PartialCorrect \<Rightarrow> PartialCorrect)"
-definition instr_comp :: "(('a::lrep) \<longmapsto> ('b::lrep)) \<Rightarrow> ( 'b \<longmapsto> ('c::lrep)) \<Rightarrow> 'a \<longmapsto> 'c"  ("_ \<nuInstrComp>/ _" [75,76] 75) 
+definition instr_comp :: "(('a::lrep) \<longmapsto> ('b::lrep)) \<Rightarrow> ( 'b \<longmapsto> ('c::lrep)) \<Rightarrow> 'a \<longmapsto> 'c"  ("_ \<then>/ _" [75,76] 75) 
   where "instr_comp f g s = bind (f s) g"
 definition nop :: " ('a::lrep) \<longmapsto> 'a" where "nop = Success" \<comment>\<open>the instruction `no-operation`\<close>
 
 lemma nop_\<nu>app: "\<^bold>p\<^bold>r\<^bold>o\<^bold>c nop \<blangle> T \<longmapsto> T \<brangle>" unfolding nop_def Procedure_def by auto
-lemma instr_comp[intro]: "\<^bold>p\<^bold>r\<^bold>o\<^bold>c f \<blangle> A \<longmapsto> B \<brangle> \<Longrightarrow> \<^bold>p\<^bold>r\<^bold>o\<^bold>c g \<blangle> B \<longmapsto> C \<brangle> \<Longrightarrow> \<^bold>p\<^bold>r\<^bold>o\<^bold>c (f \<nuInstrComp> g) \<blangle> A \<longmapsto> C \<brangle>"
+lemma instr_comp[intro]: "\<^bold>p\<^bold>r\<^bold>o\<^bold>c f \<blangle> A \<longmapsto> B \<brangle> \<Longrightarrow> \<^bold>p\<^bold>r\<^bold>o\<^bold>c g \<blangle> B \<longmapsto> C \<brangle> \<Longrightarrow> \<^bold>p\<^bold>r\<^bold>o\<^bold>c (f \<then> g) \<blangle> A \<longmapsto> C \<brangle>"
   unfolding instr_comp_def Procedure_def bind_def by (auto 0 4)
 
 
@@ -527,7 +527,7 @@ lemma reassemble_proc_0:
   unfolding CurrentConstruction_def PendingConstruction_def CodeBlock_def nop_def bind_def by (cases s) simp+
 
 lemma reassemble_proc:
-  "(\<And>s'. CodeBlock s' s f \<Longrightarrow> \<^bold>p\<^bold>e\<^bold>n\<^bold>d\<^bold>i\<^bold>n\<^bold>g g \<^bold>o\<^bold>n s' [H] \<^bold>r\<^bold>e\<^bold>s\<^bold>u\<^bold>l\<^bold>t\<^bold>s \<^bold>i\<^bold>n T) \<Longrightarrow> \<^bold>p\<^bold>e\<^bold>n\<^bold>d\<^bold>i\<^bold>n\<^bold>g (f \<nuInstrComp> g) \<^bold>o\<^bold>n s [H] \<^bold>r\<^bold>e\<^bold>s\<^bold>u\<^bold>l\<^bold>t\<^bold>s \<^bold>i\<^bold>n T"
+  "(\<And>s'. CodeBlock s' s f \<Longrightarrow> \<^bold>p\<^bold>e\<^bold>n\<^bold>d\<^bold>i\<^bold>n\<^bold>g g \<^bold>o\<^bold>n s' [H] \<^bold>r\<^bold>e\<^bold>s\<^bold>u\<^bold>l\<^bold>t\<^bold>s \<^bold>i\<^bold>n T) \<Longrightarrow> \<^bold>p\<^bold>e\<^bold>n\<^bold>d\<^bold>i\<^bold>n\<^bold>g (f \<then> g) \<^bold>o\<^bold>n s [H] \<^bold>r\<^bold>e\<^bold>s\<^bold>u\<^bold>l\<^bold>t\<^bold>s \<^bold>i\<^bold>n T"
   unfolding CurrentConstruction_def PendingConstruction_def CodeBlock_def bind_def instr_comp_def
   by force
 
